src/arch/x64/X64.Leakage_i.fst
@@ -15,19 +15,19 @@ let combine_reg_taints regs1 regs2 =
 let combine_taint_states (ts:taintState) (ts1:taintState) (ts2:taintState) =
   TaintState (combine_reg_taints ts1.regTaint ts2.regTaint) (merge_taint ts1.flagsTaint ts2.flagsTaint)
   
-let rec check_if_block_consumes_fixed_time (block:tainted_codes) (ts:taintState) : bool * taintState =
+let rec check_if_block_consumes_fixed_time (block:tainted_codes) (fuel:nat) (ts:taintState) : bool * taintState =
   match block with
   | [] -> true, ts
-  | hd::tl -> let fixedTime, ts_int = check_if_code_consumes_fixed_time hd ts in
+  | hd::tl -> let fixedTime, ts_int = check_if_code_consumes_fixed_time hd fuel ts in
     if (not fixedTime) then fixedTime, ts_int
-    else check_if_block_consumes_fixed_time tl ts_int
+    else check_if_block_consumes_fixed_time tl fuel ts_int
     
 
-and check_if_code_consumes_fixed_time (code:tainted_code) (ts:taintState) : bool * taintState =
+and check_if_code_consumes_fixed_time (code:tainted_code) (fuel:nat) (ts:taintState) : bool * taintState =
   match code with
-  | Ins ins -> check_if_ins_consumes_fixed_time ins ts
+  | Ins ins -> check_if_ins_consumes_fixed_time ins fuel ts
   
-  | Block block -> check_if_block_consumes_fixed_time block ts
+  | Block block -> check_if_block_consumes_fixed_time block fuel ts
 
   | IfElse ifCond ifTrue ifFalse ->
     let cond_taint = ifCond.ot in
@@ -42,10 +42,10 @@ and check_if_code_consumes_fixed_time (code:tainted_code) (ts:taintState) : bool
       let o2Public = operand_does_not_use_secrets (get_snd_ocmp ifCond.o) ts in
       if (not o2Public) then (false, ts)
       else
-      let validIfTrue, tsIfTrue = check_if_code_consumes_fixed_time ifTrue ts in
+      let validIfTrue, tsIfTrue = check_if_code_consumes_fixed_time ifTrue fuel ts in
       if (not validIfTrue) then (false, ts)
       else
-      let validIfFalse, tsIfFalse = check_if_code_consumes_fixed_time ifFalse ts in
+      let validIfFalse, tsIfFalse = check_if_code_consumes_fixed_time ifFalse fuel ts in
       if (not validIfFalse) then (false, ts)
       else
       (true, combine_taint_states ts tsIfTrue tsIfFalse)
@@ -75,98 +75,98 @@ and check_if_loop_consumes_fixed_time (pred:tainted_ocmp) (body:tainted_code) (t
 *)
   
 
-val lemma_equal_eval_isConstant_aux: (code1: tainted_code) -> (code2:tainted_code) -> (ts:taintState) -> (ts':taintState) -> (s1 : traceState) -> (s2:traceState) -> Lemma ((forall s. taint_eval_code code1 s == taint_eval_code code2 s) ==> 
-  isConstantTimeGivenStates code1 ts s1 s2 /\ isExplicitLeakageFreeGivenStates code1 ts ts' s1 s2 ==> isConstantTimeGivenStates code2 ts s1 s2 /\ isExplicitLeakageFreeGivenStates code2 ts ts' s1 s2)
+val lemma_equal_eval_isConstant_aux: (code1: tainted_code) -> (code2:tainted_code) -> (fuel:nat) -> (ts:taintState) -> (ts':taintState) -> (s1 : traceState) -> (s2:traceState) -> Lemma ((forall s. taint_eval_code code1 fuel s == taint_eval_code code2 fuel s) ==> 
+  isConstantTimeGivenStates code1 fuel ts s1 s2 /\ isExplicitLeakageFreeGivenStates code1 fuel ts ts' s1 s2 ==> isConstantTimeGivenStates code2 fuel ts s1 s2 /\ isExplicitLeakageFreeGivenStates code2 fuel ts ts' s1 s2)
   
-let lemma_equal_eval_isConstant_aux code1 code2 ts ts' s1 s2 = ()
+let lemma_equal_eval_isConstant_aux code1 code2 fuel ts ts' s1 s2 = ()
 
-val lemma_equal_eval_isConstant: (code1: tainted_code) -> (code2:tainted_code) -> (ts:taintState) -> (ts':taintState) -> Lemma ((forall s. taint_eval_code code1 s == taint_eval_code code2 s) ==> 
-  isConstantTime code1 ts /\ isLeakageFree code1 ts ts' ==> isConstantTime code2 ts /\ isLeakageFree code2 ts ts')
+val lemma_equal_eval_isConstant: (code1: tainted_code) -> (code2:tainted_code) -> (fuel:nat) -> (ts:taintState) -> (ts':taintState) -> Lemma ((forall s. taint_eval_code code1 s == taint_eval_code code2 s) ==> 
+  isConstantTime code1 fuel ts /\ isLeakageFree code1 fuel ts ts' ==> isConstantTime code2 fuel ts /\ isLeakageFree code2 fuel ts ts')
   
-let lemma_equal_eval_isConstant code1 code2 ts ts' = FStar.Classical.forall_intro_2 (lemma_equal_eval_isConstant_aux code1 code2 ts ts')
+let lemma_equal_eval_isConstant code1 code2 fuel ts ts' = FStar.Classical.forall_intro_2 (lemma_equal_eval_isConstant_aux code1 code2 fuel ts ts')
 
-val monotone_ok_eval: (code:tainted_code) -> (s:traceState) -> Lemma
+val monotone_ok_eval: (code:tainted_code) -> (fuel:nat) -> (s:traceState) -> Lemma
  (requires True)
- (ensures (let s' = taint_eval_code code s in
+ (ensures (let s' = taint_eval_code code fuel s in
     Some? s' /\ (Some?.v s').state.ok ==> s.state.ok))
  (decreases %[code; 0])
 
-val monotone_ok_eval_block: (codes:tainted_codes) -> (s:traceState) -> Lemma
+val monotone_ok_eval_block: (codes:tainted_codes) -> (fuel:nat) -> (s:traceState) -> Lemma
  (requires True)
- (ensures (let s' = taint_eval_codes codes s in
+ (ensures (let s' = taint_eval_codes codes fuel s in
     Some? s' /\ (Some?.v s').state.ok ==> s.state.ok))
  (decreases %[codes;1])
 
 #set-options "--z3rlimit 20"
-let rec monotone_ok_eval code s = match code with
+let rec monotone_ok_eval code fuel s = match code with
   | Ins ins -> ()
-  | Block block -> monotone_ok_eval_block block s
+  | Block block -> monotone_ok_eval_block block fuel s
   | IfElse ifCond ifTrue ifFalse ->
     let st, b = taint_eval_ocmp s ifCond in
     let st = {st with trace=BranchPredicate(b)::s.trace} in
-    if b then monotone_ok_eval ifTrue st else monotone_ok_eval ifFalse st
-  | While _ _ _ -> admit()
+    if b then monotone_ok_eval ifTrue fuel st else monotone_ok_eval ifFalse fuel st
+  | While _ _ -> admit()
 
-and monotone_ok_eval_block block s =
+and monotone_ok_eval_block block fuel s =
   match block with
   | [] -> ()
   | hd :: tl -> 
-    let s' = taint_eval_code hd s in
+    let s' = taint_eval_code hd fuel s in
     if None? s' then () else
-    monotone_ok_eval_block tl (Some?.v s');
-    monotone_ok_eval hd s
+    monotone_ok_eval_block tl fuel (Some?.v s');
+    monotone_ok_eval hd fuel s
 
-val lemma_code_explicit_leakage_free: (ts:taintState) -> (code:tainted_code) -> (s1:traceState) -> (s2:traceState) -> Lemma
+val lemma_code_explicit_leakage_free: (ts:taintState) -> (code:tainted_code) -> (fuel:nat) -> (s1:traceState) -> (s2:traceState) -> Lemma
  (requires True)
- (ensures (let b, ts' = check_if_code_consumes_fixed_time code ts in
-  (b2t b ==> isConstantTimeGivenStates code ts s1 s2 /\ isExplicitLeakageFreeGivenStates code ts ts' s1 s2)))
+ (ensures (let b, ts' = check_if_code_consumes_fixed_time code fuel ts in
+  (b2t b ==> isConstantTimeGivenStates code fuel ts s1 s2 /\ isExplicitLeakageFreeGivenStates code fuel ts ts' s1 s2)))
  (decreases %[code; 0])
 
-val lemma_block_explicit_leakage_free: (ts:taintState) -> (codes:tainted_codes) -> (s1:traceState) -> (s2:traceState) -> Lemma
+val lemma_block_explicit_leakage_free: (ts:taintState) -> (codes:tainted_codes) -> (fuel:nat) -> (s1:traceState) -> (s2:traceState) -> Lemma
  (requires True)
- (ensures (let b, ts' = check_if_block_consumes_fixed_time codes ts in
-  (b2t b ==> isConstantTimeGivenStates (Block codes) ts s1 s2 /\ isExplicitLeakageFreeGivenStates (Block codes) ts ts' s1 s2)))
+ (ensures (let b, ts' = check_if_block_consumes_fixed_time codes fuel ts in
+  (b2t b ==> isConstantTimeGivenStates (Block codes) fuel ts s1 s2 /\ isExplicitLeakageFreeGivenStates (Block codes) fuel ts ts' s1 s2)))
  (decreases %[codes;1])
 
-let rec lemma_code_explicit_leakage_free ts code s1 s2 = match code with
-  | Ins ins -> lemma_ins_leakage_free ts ins
-  | Block block -> lemma_block_explicit_leakage_free ts block s1 s2
+let rec lemma_code_explicit_leakage_free ts code fuel s1 s2 = match code with
+  | Ins ins -> lemma_ins_leakage_free ts fuel ins
+  | Block block -> lemma_block_explicit_leakage_free ts block fuel s1 s2
   | IfElse ifCond ifTrue ifFalse ->     
-    let b_fin, ts_fin = check_if_code_consumes_fixed_time code ts in
+    let b_fin, ts_fin = check_if_code_consumes_fixed_time code fuel ts in
     let st1, b1 = taint_eval_ocmp s1 ifCond in
     let st1 = {st1 with trace=BranchPredicate(b1)::s1.trace} in
     let st2, b2 = taint_eval_ocmp s2 ifCond in
     let st2 = {st2 with trace=BranchPredicate(b2)::s2.trace} in
     assert (b2t b_fin ==> constTimeInvariant ts s1 s2 /\ st1.state.ok /\ st2.state.ok ==> constTimeInvariant ts st1 st2);
-    monotone_ok_eval ifTrue st1;
-    monotone_ok_eval ifTrue st2;
-    lemma_code_explicit_leakage_free ts ifTrue st1 st2;
-    monotone_ok_eval ifFalse st1;
-    monotone_ok_eval ifFalse st2;
-    lemma_code_explicit_leakage_free ts ifFalse st1 st2;
+    monotone_ok_eval ifTrue fuel st1;
+    monotone_ok_eval ifTrue fuel st2;
+    lemma_code_explicit_leakage_free ts ifTrue fuel st1 st2;
+    monotone_ok_eval ifFalse fuel st1;
+    monotone_ok_eval ifFalse fuel st2;
+    lemma_code_explicit_leakage_free ts ifFalse fuel st1 st2;
     ()
   | _ -> ()
 
-and lemma_block_explicit_leakage_free ts block s1 s2 = match block with
+and lemma_block_explicit_leakage_free ts block fuel s1 s2 = match block with
   | [] -> ()
   | hd :: tl ->
-    let b, ts' = check_if_code_consumes_fixed_time hd ts in
-    lemma_code_explicit_leakage_free ts hd s1 s2;
-    let s'1 = taint_eval_code hd s1 in
-    let s'2 = taint_eval_code hd s2 in
+    let b, ts' = check_if_code_consumes_fixed_time hd fuel ts in
+    lemma_code_explicit_leakage_free ts hd fuel s1 s2;
+    let s'1 = taint_eval_code hd fuel s1 in
+    let s'2 = taint_eval_code hd fuel s2 in
     if None? s'1 || None? s'2 then ()
     else
     let s'1 = Some?.v s'1 in
     let s'2 = Some?.v s'2 in
-    lemma_block_explicit_leakage_free ts' tl s'1 s'2;
-    monotone_ok_eval (Block tl) s'1;
-    monotone_ok_eval (Block tl) s'2
+    lemma_block_explicit_leakage_free ts' tl fuel s'1 s'2;
+    monotone_ok_eval (Block tl) fuel s'1;
+    monotone_ok_eval (Block tl) fuel s'2
 
-val lemma_code_leakage_free: (ts:taintState) -> (code:tainted_code) -> Lemma
- (let b, ts' = check_if_code_consumes_fixed_time code ts in
-  (b2t b ==> isConstantTime code ts /\ isLeakageFree code ts ts'))
+val lemma_code_leakage_free: (ts:taintState) -> (code:tainted_code) -> (fuel:nat) -> Lemma
+ (let b, ts' = check_if_code_consumes_fixed_time code fuel ts in
+  (b2t b ==> isConstantTime code fuel ts /\ isLeakageFree code fuel ts ts'))
 
-let lemma_code_leakage_free ts code = FStar.Classical.forall_intro_2 (lemma_code_explicit_leakage_free ts code)
+let lemma_code_leakage_free ts code fuel = FStar.Classical.forall_intro_2 (lemma_code_explicit_leakage_free ts code fuel)
   
 (* val check_if_code_is_leakage_free: (code:tainted_code) -> (ts:taintState) -> (tsExpected:taintState) -> (b:bool{b ==> isLeakageFree code ts tsExpected
 	 /\ b ==> isConstantTime code ts})
